theories/zoo_partition/partition__code.v
@@ -125,7 +125,7 @@ Definition partition_cardinal : val :=
   fun: "elt" =>
     "elt".{class_}.{len}.
 
-Definition partition_record_0 : val :=
+Definition partition_record₀ : val :=
   fun: "split_list" "elt" =>
     let: "class_" := "elt".{class_} in
     if: partition_class_is_singleton "class_" or "elt".{seen} then (
@@ -152,9 +152,9 @@ Definition partition_record_0 : val :=
 
 Definition partition_record : val :=
   fun: "elts" =>
-    lst_foldl partition_record_0 [] "elts".
+    lst_foldl partition_record₀ [] "elts".
 
-Definition partition_split_0 : val :=
+Definition partition_split₀ : val :=
   fun: "class_" =>
     let: "first" := "class_".{first} in
     let: "split" := "class_".{split} in
@@ -177,7 +177,7 @@ Definition partition_split_0 : val :=
 
 Definition partition_split : val :=
   fun: "split_list" =>
-    lst_iter partition_split_0 "split_list".
+    lst_iter partition_split₀ "split_list".
 
 Definition partition_refine : val :=
   fun: "elts" =>
