theories/zoo_saturn/ws_bdeque_1.v
@@ -1867,7 +1867,7 @@ Module base.
       | PopEmptyishWinner v
       | PopEmptyishLoser
       | PopSuperempty.
-    #[local] Lemma ws_bdeque_1_pop_0𑁒spec {t γ} (state : pop_state) {stable} back ws front_cache us id (back_ : Z) :
+    #[local] Lemma ws_bdeque_1_pop₀𑁒spec {t γ} (state : pop_state) {stable} back ws front_cache us id (back_ : Z) :
       back_ = back →
       {{{
         inv' t γ ∗
@@ -1892,7 +1892,7 @@ Module base.
             ⌜front = S back⌝
         end
       }}}
-        ws_bdeque_1_pop_0 #t #id #back_
+        ws_bdeque_1_pop₀ #t #id #back_
       {{{
         o back front_cache i us
       , RET o;
@@ -2045,7 +2045,7 @@ Module base.
         { iExists Superempty. iFrameSteps. }
         iIntros "!> {%- Hcapacity Hfront_cache Hus Hback}".
 
-        wp_apply+ (ws_bdeque_1_pop_0𑁒spec PopSuperempty (back - 1) with "[- HΦ]"); [lia | iFrameSteps |].
+        wp_apply+ (ws_bdeque_1_pop₀𑁒spec PopSuperempty (back - 1) with "[- HΦ]"); [lia | iFrameSteps |].
         iSteps.
       }
 
@@ -2085,7 +2085,7 @@ Module base.
           { iExists Emptyish. iFrameSteps. }
           iIntros "!> {%- Hcapacity Hfront_cache Hus Hback Hus_lookup}".
 
-          wp_apply+ (ws_bdeque_1_pop_0𑁒spec (PopEmptyishWinner v) front1 with "[- HΦ]"); [lia | iFrameSteps |].
+          wp_apply+ (ws_bdeque_1_pop₀𑁒spec (PopEmptyishWinner v) front1 with "[- HΦ]"); [lia | iFrameSteps |].
           iSteps.
 
         + iDestruct "Hwinner" as "[(:winner) | Hwinner]".
@@ -2101,7 +2101,7 @@ Module base.
             { iExists Emptyish. iFrameSteps. }
             iIntros "!> {%- Hcapacity Hfront_cache Hus Hus_lookup}".
 
-            wp_apply+ (ws_bdeque_1_pop_0𑁒spec (PopEmptyishWinner v) front1 with "[- HΦ]"); [lia | iFrameSteps |].
+            wp_apply+ (ws_bdeque_1_pop₀𑁒spec (PopEmptyishWinner v) front1 with "[- HΦ]"); [lia | iFrameSteps |].
             iSteps.
           }
 
@@ -2124,7 +2124,7 @@ Module base.
           { iExists Emptyish. iFrameStep 7. iExists P. iSteps. }
           iIntros "!> {%- Hcapacity Hfront_cache Hus Hbranch2}".
 
-          wp_apply+ (ws_bdeque_1_pop_0𑁒spec PopEmptyishLoser front1 with "[- HΦ]"); [lia | iFrameSteps |].
+          wp_apply+ (ws_bdeque_1_pop₀𑁒spec PopEmptyishLoser front1 with "[- HΦ]"); [lia | iFrameSteps |].
           iSteps.
 
       - iMod (owner_update Stable (back - 1) with "Howner₁ Howner₂") as "(Howner₁ & Howner₂)".
@@ -2148,7 +2148,7 @@ Module base.
         }
         iIntros "!> {%- Hcapacity Hfront_cache Hus Hback Hus_lookup}".
 
-        wp_apply+ (ws_bdeque_1_pop_0𑁒spec (PopNonempty v) (back - 1) with "[- HΦ]"); [lia | iFrameSteps |].
+        wp_apply+ (ws_bdeque_1_pop₀𑁒spec (PopNonempty v) (back - 1) with "[- HΦ]"); [lia | iFrameSteps |].
         iSteps.
     Qed.
   End ws_bdeque_1_G.
