theories/zoo_std/lst.v
@@ -199,7 +199,7 @@ Section zoo_G.
       wp_apply ("IH" with "[%] [//] [//] [//] HΦ"); first lia.
   Qed.
 
-  #[local] Lemma lst_initi_0𑁒spec vs_left Ψ sz fn i :
+  #[local] Lemma lst_initi₀𑁒spec vs_left Ψ sz fn i :
     i ≤ ₊sz →
     i = length vs_left →
     {{{
@@ -213,7 +213,7 @@ Section zoo_G.
         }}
       )
     }}}
-      lst_initi_0 #sz fn #i
+      lst_initi₀ #sz fn #i
     {{{
       t vs_right
     , RET t;
@@ -262,7 +262,7 @@ Section zoo_G.
   Proof.
     iIntros "%Φ (HΨ & #Hfn) HΦ".
     wp_rec.
-    wp_apply+ (lst_initi_0𑁒spec [] Ψ with "[$HΨ $Hfn] HΦ"); simpl; lia.
+    wp_apply+ (lst_initi₀𑁒spec [] Ψ with "[$HΨ $Hfn] HΦ"); simpl; lia.
   Qed.
   Lemma lst_initi𑁒spec' Ψ sz fn :
     {{{
@@ -459,7 +459,7 @@ Section zoo_G.
     iSteps.
   Qed.
 
-  #[local] Lemma lst_foldli_0𑁒spec vs_left Ψ vs fn i acc t vs_right :
+  #[local] Lemma lst_foldli₀𑁒spec vs_left Ψ vs fn i acc t vs_right :
     vs = vs_left ++ vs_right →
     i = length vs_left →
     lst_model' t vs_right →
@@ -474,7 +474,7 @@ Section zoo_G.
         }}
       )
     }}}
-      lst_foldli_0 fn #i acc t
+      lst_foldli₀ fn #i acc t
     {{{
       acc
     , RET acc;
@@ -519,7 +519,7 @@ Section zoo_G.
     iIntros "%Ht %Φ (HΨ & #Hfn) HΦ".
     wp_rec.
     rewrite -Nat2Z.inj_0.
-    wp_apply+ (lst_foldli_0𑁒spec [] Ψ with "[$HΨ $Hfn //] HΦ"); done.
+    wp_apply+ (lst_foldli₀𑁒spec [] Ψ with "[$HΨ $Hfn //] HΦ"); done.
   Qed.
   Lemma lst_foldli𑁒spec' Ψ fn acc t vs :
     lst_model' t vs →
@@ -604,7 +604,7 @@ Section zoo_G.
     iSteps.
   Qed.
 
-  #[local] Lemma lst_foldri_0𑁒spec vs_left Ψ vs fn i t vs_right acc :
+  #[local] Lemma lst_foldri₀𑁒spec vs_left Ψ vs fn i t vs_right acc :
     vs = vs_left ++ vs_right →
     i = length vs_left →
     lst_model' t vs_right →
@@ -619,7 +619,7 @@ Section zoo_G.
         }}
       )
     }}}
-      lst_foldri_0 fn #i t acc
+      lst_foldri₀ fn #i t acc
     {{{
       acc
     , RET acc;
@@ -664,7 +664,7 @@ Section zoo_G.
     iIntros "%Ht %Φ (HΨ & #Hfn) HΦ".
     wp_rec.
     rewrite -Nat2Z.inj_0.
-    wp_apply+ (lst_foldri_0𑁒spec [] Ψ with "[$HΨ $Hfn] HΦ"); done.
+    wp_apply+ (lst_foldri₀𑁒spec [] Ψ with "[$HΨ $Hfn] HΦ"); done.
   Qed.
   Lemma lst_foldri𑁒spec' Ψ fn t vs acc :
     lst_model' t vs →
@@ -1064,7 +1064,7 @@ Section zoo_G.
     iSteps.
   Qed.
 
-  #[local] Lemma lst_mapi_0𑁒spec vs_left ws_left Ψ vs fn i t vs_right :
+  #[local] Lemma lst_mapi₀𑁒spec vs_left ws_left Ψ vs fn i t vs_right :
     vs = vs_left ++ vs_right →
     i = length vs_left →
     i = length ws_left →
@@ -1080,7 +1080,7 @@ Section zoo_G.
         }}
       )
     }}}
-      lst_mapi_0 fn #i t
+      lst_mapi₀ fn #i t
     {{{
       t' ws_right
     , RET t';
@@ -1132,7 +1132,7 @@ Section zoo_G.
   Proof.
     iIntros "%Ht %Φ (HΨ & #Hfn) HΦ".
     wp_rec.
-    wp_apply+ (lst_mapi_0𑁒spec [] [] Ψ with "[$HΨ $Hfn]"); [done.. |].
+    wp_apply+ (lst_mapi₀𑁒spec [] [] Ψ with "[$HΨ $Hfn]"); [done.. |].
     iSteps.
   Qed.
   Lemma lst_mapi𑁒spec' Ψ fn t vs :
